Source/DafnyCore/Rewriters/RewriterCollection.cs
@@ -51,10 +51,6 @@ public static class RewriterCollection {
       result.Add(new AutoRevealFunctionDependencies(reporter));
     }
 
-    if (reporter.Options.Get(CommonOptionBag.CheckInvariants)) {
-      result.Add(new InvariantRewriter(program, reporter));
-    }
-
     foreach (var plugin in reporter.Options.Plugins) {
       result.AddRange(plugin.GetRewriters(reporter));
     }
