Source/DafnyCore/Verifier/BoogieGenerator.Functions.Wellformedness.cs
@@ -121,6 +121,11 @@ public partial class BoogieGenerator {
       // of them), do the postponed reads checks.
       delayer.DoWithDelayedReadsChecks(false, wfo => {
         builder.Add(new CommentCmd("Check well-formedness of preconditions, and then assume them"));
+        // If the object has an invariant and f is an instance function, then it can be assumed to check the well-formedness of its preconditions (see well-formedness check for methods for the general principle)
+        if (generator.options.Get(CommonOptionBag.CheckInvariants) && f is not Invariant and { IsStatic: false, EnclosingClass: TopLevelDeclWithMembers { Invariant: { } invariant } }) {
+          var assertion = invariant.Mention(f.Origin, new ThisExpr(f), generator.program.SystemModuleManager);
+          generator.CheckWellformedAndAssume(assertion, wfo, locals, builder, etran, "object invariant as precondition");
+        }
         foreach (AttributedExpression require in ConjunctsOf(f.Req)) {
           if (require.Label != null) {
             require.Label.E = (f is TwoStateFunction ? ordinaryEtran : etran.Old).TrExpr(require.E);
@@ -324,10 +329,17 @@ public partial class BoogieGenerator {
           postCheckBuilder.Add(TrAssumeCmd(f.Result.Origin, wh));
         }
       }
+
+      var wfo = new WFOptions(f, doReadsChecks);
+      // If the object has an invariant and f is an instance function, then it can be assumed to check the well-formedness of its postconditions (see preconditions case above)
+      if (generator.options.Get(CommonOptionBag.CheckInvariants) && f is not Invariant and { IsStatic: false, EnclosingClass: TopLevelDeclWithMembers { Invariant: { } invariant } }) {
+        var assertion = invariant.Mention(f.Origin, new ThisExpr(f), generator.program.SystemModuleManager);
+        generator.CheckWellformedAndAssume(assertion, wfo, locals, postCheckBuilder, etran, "object invariant as precondition");
+      }
       // Now for the ensures clauses
       foreach (AttributedExpression p in f.Ens) {
         // assume the postcondition for the benefit of checking the remaining postconditions
-        generator.CheckWellformedAndAssume(p.E, new WFOptions(f, doReadsChecks), locals, postCheckBuilder, etran, "ensures clause");
+        generator.CheckWellformedAndAssume(p.E, wfo, locals, postCheckBuilder, etran, "ensures clause");
       }
 
       postCheckBuilder.Add(TrAssumeCmd(f.Origin, Expr.False));
