Source/IntegrationTests/TestFiles/LitTests/LitTest/invariants/Account.dfy
@@ -1,3 +1,6 @@
+// RUN: %verify --type-system-refresh --check-invariants "%s" > "%t"
+// RUN: %diff "%s.expect" "%t"
+
 class Account {
   var credit: nat
   var debit: nat
