Source/IntegrationTests/TestFiles/LitTests/LitTest/invariants/TempInvariantBreakingError.dfy
@@ -1,4 +1,4 @@
-// RUN: %verify --type-system-refresh --check-invariants "%s" > "%t"
+// RUN: %exits-with 4 %verify --type-system-refresh --check-invariants "%s" > "%t"
 // RUN: %diff "%s.expect" "%t"
 
 class C {
@@ -7,7 +7,7 @@ class C {
   invariant x != 0
 
   constructor() {
-     x := 1; 
+     x := 1;
      x := 0; // breaking the invariant here is fine
      x := 1; // as long at it is satisfied at the end
   }
@@ -16,9 +16,9 @@ class C {
     modifies this
   {
      x := 0; // temporarily breaking the invariant outside the constructor is allowed
-     //UseInvariant(this); // error: invariant doesn't hold here (force checked, since this is open)
+     UseInvariant(this); // error: invariant doesn't hold here (force checked, since this is open)
      var me := this;
-     //UseInvariant(me); //  error: same as above (this can be copied as much as you want)
+     UseInvariant(me); //  error: same as above (this can be copied as much as you want)
      x := 1;
   }
  
@@ -35,6 +35,6 @@ class C {
   static method External2(c: C)
     modifies c
   {
-     //c.x := 0; // verifier error: c's invariant cannot be re-established
+     c.x := 0; // verifier error: c's invariant cannot be re-established
   }
 }
